MECMAR/tactics/Retrieve.v
@@ -1,0 +1,18 @@
+Require Import Ltac2.Ltac2.
+From Ltac2 Require Import Control Pattern List.
+
+(** TODO: once updated to a newer version (1.19.0?) supporting https://github.com/coq/coq/pull/18690,
+          remove and use builtin.
+*)
+Ltac2 numgoals (_: unit): int :=
+  1.
+
+Ltac2 retrieve (pat: pattern) (into: ident): unit :=
+  let hyp_patterns := (None, (Pattern.MatchPattern, pat)) :: [] in
+  let goal_pattern := (Pattern.MatchPattern, pat:(_)) in
+  (* TODO: change to lazy match, if possible *)
+  let (a, _, _, _, _) := Pattern.matches_goal false hyp_patterns goal_pattern in
+  if Bool.neg (Int.equal (numgoals ()) 1) then Control.throw_invalid_argument "Multiple hypothese match the pattern" else ();
+  let h := Array.get a 0 in
+  Std.rename ((h, into) :: []).
+Ltac2 Notation "retrieve" pat(pattern) "as" into(ident) := retrieve pat into.
