MECMAR/utils/Typeclasses.v
@@ -8,6 +8,9 @@ Module EqDec.
 
   Lemma inversion_true {T: Type} `{type T}: forall (l r: T), eqb l r = true <-> l = r.
   Proof. intros. unfold eqb. destruct (eq_dec l r) eqn:Eq; split; easy. Qed.
+
+  Lemma inversion_false {T: Type} `{type T}: forall (l r: T), eqb l r = false <-> l <> r.
+  Proof. intros. unfold eqb. destruct (eq_dec l r) eqn:Eq; split; easy. Qed.
 End EqDec.
 Notation EqDec := EqDec.type.
 Infix "=?=" := EqDec.eq_dec (at level 37, no associativity).
@@ -19,5 +22,6 @@ Instance eqdec_bool: EqDec bool := { eq_dec := Bool.bool_dec }.
 Instance eqdec_nat: EqDec nat := { eq_dec := Nat.eq_dec }.
 Instance eqdec_string: EqDec String.string := { eq_dec := String.string_dec }.
 #[refine] Instance eqdec_positive: EqDec positive := {}. decide equality. Defined.
+#[refine] Instance eqdec_Z: EqDec Z := {}. decide equality; apply EqDec.eq_dec. Defined.
 #[refine] Instance eqdec_option {T: Type} `{EqDec T}: EqDec (option T) := {}. decide equality; apply EqDec.eq_dec. Defined.
 #[refine] Instance eqdec_list {T: Type} `{EqDec T}: EqDec (list T) := {}. decide equality; apply EqDec.eq_dec. Defined.
